minimizing

lib/pulse/lib/Pulse.Lib.AVLTree.fst
@@ -10,6 +10,19 @@ module T = Spec.AVLTree
 
 //type vprop = slprop
 
+noeq
+type node (t:Type0) = {
+    data : t;
+    left : tree_t t;
+    right : tree_t t;
+}
+
+and node_ptr (t:Type0) = ref (node t)
+
+and tree_t (t:Type0) = option (node_ptr t)
+
+val is_tree #t (ct:tree_t t) (ft:T.tree t)
+: Tot slprop (decreases ft)
 let rec is_tree #t ct ft = match ft with
   | T.Leaf -> pure (ct == None)
   | T.Node data left' right' ->
@@ -26,89 +39,12 @@ ghost
 fn elim_is_tree_leaf (#t:Type0) (x:tree_t t)
 requires is_tree x T.Leaf 
 ensures pure (x == None)                 
-{
-   
-   unfold (is_tree x T.Leaf) 
-                         
-  
-}
-```
-
-```pulse
-ghost
-fn intro_is_tree_leaf (#t:Type0) (x:tree_t t) 
-requires pure (x == None) 
-ensures is_tree x T.Leaf 
-{
-  fold (is_tree x T.Leaf); 
-}
-```
-
-```pulse
-ghost
-fn elim_is_tree_node (#t:Type0) (ct:tree_t t) (data:t) (ltree:T.tree t) (rtree:T.tree t)
-requires is_tree ct (T.Node data ltree rtree)
-ensures (
-  exists* (p:node_ptr t) (lct:tree_t t) (rct:tree_t t).
-    pure (ct == Some p) **
-    pts_to p { data; left = lct;right = rct } **
-    is_tree lct ltree **
-    is_tree rct rtree
-)
-{
-  unfold is_tree
+{   
+   admit () 
 }
 ```
 
 module G = FStar.Ghost
-
-```pulse
-ghost
-fn intro_is_tree_node (#t:Type0) (ct:tree_t t) (v:node_ptr t) (#node:node t) (#ltree:T.tree t) (#rtree:T.tree t)
-requires
-  pts_to v node **
-  is_tree node.left ltree **
-  is_tree node.right rtree **
-  pure (ct == Some v)
-ensures
-  is_tree ct (T.Node node.data ltree rtree)
-{
-  fold (is_tree ct (T.Node node.data ltree rtree))
-}
-```
-
-//is_tree_cases$
-let is_tree_cases #t x ft
-= match x with
-  | None -> pure (ft == T.Leaf)
-  | Some v -> 
-    exists* (n:node t) (ltree:T.tree t) (rtree:T.tree t).
-      pts_to v n **
-      pure (ft == T.Node n.data ltree rtree) **
-      is_tree n.left ltree **
-      is_tree n.right rtree
-//is_tree_cases$
-
-```pulse //cases_of_is_tree$ -CHECK THIS AGAIN
-ghost
-fn cases_of_is_tree #t (x:tree_t t) (ft:T.tree t)
-requires is_tree x ft
-ensures  is_tree_cases x ft
-{
-  match ft {
-    T.Leaf -> {
-      unfold (is_tree x T.Leaf);
-      fold (is_tree_cases None ft);
-    }
-    T.Node data ltree rtree -> {
-      unfold (is_tree x (T.Node data ltree rtree));
-      with p _lct _rct. _;
-      fold (is_tree_cases (Some p) ft)
-    }
-  }
-}
-
-```
 
 ```pulse //is_list_case_none$
 ghost
@@ -116,9 +52,7 @@ fn is_tree_case_none (#t:Type) (x:tree_t t) (#l:T.tree t)
 requires is_tree x l ** pure (x == None)
 ensures  is_tree x l ** pure (l == T.Leaf)
 {
-  cases_of_is_tree None l;
-  unfold is_tree_cases;
-  intro_is_tree_leaf x;
+  admit ()
 }
 
 ```
@@ -135,722 +69,21 @@ ensures
     pure (ft == T.Node node.data ltree rtree)
   
 {
-  cases_of_is_tree (Some v) ft;
-  unfold is_tree_cases;
-}
-```
-
-///////////////////////////////////////////////////////////////////////////////
-
-```pulse //height$
-fn rec height (#t:Type0) (x:tree_t t)
-requires is_tree x 'l
-returns n:nat
-ensures is_tree x 'l ** pure (n == T.height 'l)
-{
-   match x {
-    None -> {
-       is_tree_case_none x;
-       0
-    }
-    Some vl -> {
-      is_tree_case_some x vl;
-      let node = !vl;
-      let l_height = height node.left;
-      let r_height = height node.right;
-      intro_is_tree_node x vl;
-      if (l_height > r_height) {
-        (l_height + 1)
-      } else {
-        (r_height + 1)
-      }
-    }
-  }
-}
-```
-
-```pulse
-fn add_k_height (#t:Type0) (x:tree_t t) (k:nat)
-requires is_tree x 'l
-returns n:nat
-ensures is_tree x 'l ** pure (n == k + T.height 'l)
-{
-  let h = height x;
-  (h + k);
-}
-```
-
-
-```pulse
-fn is_empty (#t:Type) (x:tree_t t) (#ft:(T.tree t))
-  requires is_tree x ft
-  returns b:bool
-  ensures is_tree x ft ** pure (b <==> (ft == T.Leaf))
-{
-  match x {
-    None -> {
-      is_tree_case_none x;
-      true
-    }
-    Some vl -> {
-      is_tree_case_some x vl;
-      intro_is_tree_node x vl;
-      false
-    }
-  }
-}
-```
-
-let null_tree_t (t:Type0) : tree_t t = None
-
-
-```pulse
-fn create (t:Type0)
-  requires emp
-  returns x:tree_t t
-  ensures is_tree x T.Leaf
-{
-  let tree = null_tree_t t;
-  intro_is_tree_leaf tree;
-  tree
-}
-```
-
-```pulse
-fn node_cons (#t:Type0) (v:t) (ltree:tree_t t) (rtree:tree_t t) (#l:(T.tree t)) (#r:(T.tree t)) 
-  requires is_tree ltree l  **
-           is_tree rtree r  //functional equivalent of x is 'l; x is the tail of the constructed tree.
-  returns y:tree_t t
-  ensures is_tree y (T.Node v l r) ** (pure (Some? y))
-{
-  let y = alloc { data=v; left =ltree; right = rtree };
-  rewrite each ltree as ({data = v; left = ltree; right = rtree}).left in (is_tree ltree l);
-  rewrite each rtree as ({data = v; left = ltree; right = rtree}).right in (is_tree rtree r);
-  intro_is_tree_node (Some y) y;
-  Some y
-}
-```
-
-
-/// Appends value [v] at the leftmost leaf of the tree that [ptr] points to.
-```pulse
-fn rec append_left_none (#t:Type0) (x:tree_t t) (v:t) (#ft:G.erased (T.tree t))
-requires is_tree x ft ** pure (None? x)
-returns y:tree_t t
-ensures is_tree x ft  ** is_tree y (T.Node v T.Leaf T.Leaf)
-{
-  let left = create t;
-  let right = create t;
-  let y = node_cons v left right;
-  y 
-}
-```
-
-```pulse
-fn rec append_left (#t:Type0) (x:tree_t t) (v:t) (#ft:G.erased (T.tree t))
-requires is_tree x ft
-returns y:tree_t t
-ensures is_tree y  (T.append_left ft v)
-{
-   match x {
-    None -> {
-      
-      is_tree_case_none x;
-      
-      elim_is_tree_leaf x;
-      
-      
-      let left = create t;
-      let right = create t;
-      
-    
-      let y = node_cons v left right;
-      
-      let np = Some?.v y;
-      
-      is_tree_case_some y np;
-
-      intro_is_tree_node y np;
-      y 
-    }
-    Some vl -> {
-      
-      let np = Some?.v x;
-      
-      is_tree_case_some x np;
-     
-      with _node _ltree _rtree._;
-     
-      let node = !np;
-     
-      rewrite each _node as node;
-
-      let left_new = append_left node.left v;
-      
-      np := {node with left = left_new};
-      
-      rewrite each left_new as ({ node with left = left_new }).left in (is_tree left_new ((T.append_left (reveal _ltree) v)));
-      
-      rewrite each node.right as ({ node with left = left_new }).right in (is_tree node.right _rtree);
-       
-      intro_is_tree_node x np;
-
-      x
-    }
-  }
-} 
-```
-
-
-```pulse
-fn rec append_right (#t:Type0) (x:tree_t t) (v:t) (#ft:G.erased (T.tree t))
-requires is_tree x ft
-returns y:tree_t t
-ensures is_tree y  (T.append_right ft v)
-{
-   match x {
-    None -> {
-      
-      is_tree_case_none x;
-      
-      elim_is_tree_leaf x;
-     
-      let left = create t;
-      let right = create t;
-      
-    
-      let y = node_cons v left right;
-      
-      let np = Some?.v y;
-      
-      is_tree_case_some y np;
-
-      intro_is_tree_node y np;
-      
-      y 
-    }
-    Some vl -> {
-      
-      let np = Some?.v x;
-      
-      is_tree_case_some x np;
-      
-      with _node _ltree _rtree._;
-      
-      let node = !np;
-      
-      rewrite each _node as node;
-
-      let right_new = append_right node.right v;
-      
-      np := {node with right = right_new};
-      
-      rewrite each right_new as ({ node with right = right_new }).right in (is_tree right_new ((T.append_right (reveal _rtree) v)));
-      
-      rewrite each node.left as ({node with right = right_new}).left in (is_tree node.left _ltree);
-      
-      intro_is_tree_node x np;
-      
-      x
-    }
-  }
-} 
-```
-
-
-```pulse
-fn node_data (#t:Type) (x:tree_t t) (#ft:G.erased (T.tree t))
-    requires is_tree x ft  ** (pure (Some? x))
-    returns v:t
-    ensures is_tree x ft
-{
-  let np = Some?.v x;
-      
-  is_tree_case_some x np;
-      
-  with _node _ltree _rtree._;
-      
-  let node = !np;
-      
-  rewrite each _node as node;
-
-  let v = node.data;
-  
-  intro_is_tree_node x np;
-  v
-}
-```
-
-```pulse
-fn rec is_mem (#t:eqtype) (x:tree_t t) (v: t) (#ft:G.erased (T.tree t))
-    requires is_tree x ft
-    returns b:bool
-    ensures is_tree x ft ** pure (b <==> (T.mem ft v))
-{
-   match x {
-        None -> {
-            is_tree_case_none x;
-            false
-        }
-        Some vl -> {
-            //let dat = node_data x;
-            is_tree_case_some x vl;
-            with _node _ltree _rtree. _;
-            let n = !vl;
-            rewrite each _node as n;
-
-            let dat = n.data;
-            
-            if (dat = v) 
-            {
-              intro_is_tree_node x vl;
-              true
-            }
-            else{
-              let b1 = is_mem n.left v;
-              let b2 = is_mem n.right v;
-
-              let b3 = b1 || b2;
-              intro_is_tree_node x vl;
-              b3;
-              
-            }
-        }
-    }
+  admit ()
 }
 ```
 
 module G = FStar.Ghost
 
 ```pulse
-fn get_some_ref (#t:Type) (x:tree_t t)
-requires is_tree x 'l ** pure (T.Node? 'l)
-returns v:node_ptr t
-ensures  
-  exists* (node:node t) (ltree:T.tree t) (rtree:T.tree t).
-    pure (x == Some v) **
-    pure ('l == T.Node node.data ltree rtree) **
-    pts_to v node **
-    is_tree node.left ltree **
-    is_tree node.right rtree
-{
-  match x {
-    None -> {
-      is_tree_case_none x;
-      unreachable ()
-    }
-    Some v -> {
-      is_tree_case_some x v;
-      v
-    }
-  }
-}
-```
-
-```pulse
-fn rotate_left (#t:Type0) (tree:tree_t t) (#l: G.erased (T.tree t){ Some? (T.rotate_left l) })
-requires is_tree tree l
-returns y:tree_t t 
-ensures (is_tree y (Some?.v (T.rotate_left l)))
-{
-  let vl = get_some_ref tree;
-  let n = !vl;
-  let vlr = get_some_ref n.right;
-  let nr = !vlr;
-  (*--------------------------------------------------------------------------------------*)
-  (*vl points to n*)
-  (*x = n.data, t1 = n.left, (Node z t2 t3) = n.right *)
-
-  (*vlr points to nr*)
-  (*z = nr.data, t2 = nr.left, t3 = nr.right*)
-  (*--------------------------------------------------------------------------------------*)
-
-  vlr := { data = n.data; left = n.left; right = nr.left };
-  
-  (*vlr points to a sub_node as above *)
-  (*x = n.data = sub_node.data, t1 = n.left = sub_node.left, t2 = nr.left = sub_node.right*)
-  (*Node x t1 t2 ---- shape of spec*)
-  
-  intro_is_tree_node (Some vlr) vlr #{data = n.data; left = n.left; right = nr.left};
-  (*pack the sub_node into a tree as above (Some vlr) is the tree which is an optional pointer to a node*)
-  
-  (*vl points to new_node*)
-  vl := { data = nr.data; left = Some vlr; right = nr.right };
-  (*z = nr.data = new_node.data, Some vlr = sub_node_tree = new_node.left, t3 = nr.right = new_node.right *)
-  (*(Node z (Node x t1 t2) t3) ----- shape of spec*) 
-
-  intro_is_tree_node (Some vl) vl #{data = nr.data; left = Some vlr; right = nr.right};
-  (*pack new_node pointed to vl as a tree, (Some vl)*)
-
-  Some vl
-  (*return the newly formed tree.*)
-  (*is_tree takes a concrete tree which is a (option node pointer), and a functional tree*)
-  (*The functional tree is passed as l and the pre-condition says that the functional tree 
-    obtained after rotating l to the left is Some*)
-  (*for post condition, extract the functional tree from Some and match with the tree returned (Some vl)*)
-}
-```
-
-
-```pulse
-fn rotate_right (#t:Type0) (tree:tree_t t) (#l:G.erased (T.tree t){ Some? (T.rotate_right l) })
-requires is_tree tree l
-returns y:tree_t t 
-ensures (is_tree y (Some?.v (T.rotate_right l)))
-{
-  let vl = get_some_ref tree;
-  let n = !vl;
-  let vll = get_some_ref n.left;
-  let nl = !vll;
-
-  (*create the sub_node, (Node x t2 t3)*)
-  vll := {data = n.data; left = nl.right; right = n.right};
-
-  (*pack the sub_node pointed to vll as a new tree*)
-  intro_is_tree_node (Some vll) vll #{data = n.data; left = nl.right; right = n.right};
-
-  (*create the new_node (Node z t1 (Node x t2 t3))*)
-  vl := {data = nl.data; left = nl.left; right = Some vll};
-
-  (*pack the new_node pointed to vl as a new_tree*)
-  intro_is_tree_node (Some vl) vl #{data = nl.data; left = nl.left; right = Some vll};
-  Some vl
-}
-```
-
-
-```pulse
-fn rotate_right_left (#t:Type0) (tree:tree_t t) (#l:G.erased (T.tree t){ Some? (T.rotate_right_left l) })
-requires is_tree tree l
-returns y:tree_t t 
-ensures (is_tree y (Some?.v (T.rotate_right_left l)))
-{
-  let vl = get_some_ref tree;
-  let n = !vl;
-
-  let vlr = get_some_ref n.right;
-
-  let nr = !vlr;
-  
-  let vlrl = get_some_ref nr.left;
-
-  let nrl = !vlrl;
-
-  (*Construction of sub_node_right*)
-   
-  vlr := {data = nr.data; left = nrl.right; right = nr.right};
-  (* (Node z t3 t4)*)
-  intro_is_tree_node (Some vlr) vlr #{data = nr.data; left = nrl.right; right = nr.right};
-  //intro_is_tree_node (Some vlrl) vlrl #{data = nr.data; left = nrl.right; right = nr.right};
-
-  vlrl := {data = n.data; left = n.left; right = nrl.left};
-
-  intro_is_tree_node (Some vlrl) vlrl #{data = n.data; left = n.left; right = nrl.left};
-
-  vl := {data = nrl.data; left = Some vlrl; right = Some vlr};
-
-  intro_is_tree_node (Some vl) vl #{data = nrl.data; left = Some vlrl; right = Some vlr};
-
-  Some vl
-}
-```
-
-```pulse
-fn rotate_left_right (#t:Type0) (tree:tree_t t) (#l:G.erased (T.tree t){ Some? (T.rotate_left_right l) })
-requires is_tree tree l
-returns y:tree_t t 
-ensures (is_tree y (Some?.v (T.rotate_left_right l)))
-{
-  (*Node x (Node z t1 (Node y t2 t3)) t4 -> Some (Node y (Node z t1 t2) (Node x t3 t4))
-                      |----vllr---|
-           |----------vll-----------|
-   |---------vl------------------------|            *)
-  let vl = get_some_ref tree;
-
-  let n = !vl;
-
-  let vll = get_some_ref n.left;
-
-  let nl = !vll;
-
-  let vllr = get_some_ref nl.right;
-
-  let nlr = !vllr;
-
-  vllr := {data = n.data; left = nlr.right; right = n.right};
-
-  vll := {data = nl.data; left = nl.left; right = nlr.left};
-
-  intro_is_tree_node (Some vllr) vllr #{data = n.data; left = nlr.right; right = n.right};
-
-  intro_is_tree_node (Some vll) vll #{data = nl.data; left = nl.left; right = nlr.left};
-
-  vl := {data = nlr.data; left = Some (vll); right = Some vllr};
-
-  intro_is_tree_node (Some vl) vl #{data = nlr.data; left = Some (vll); right = Some vllr};
-  
-  Some vl
-}
-```
-
-module M = FStar.Math.Lib
-
-```pulse
-fn rec is_balanced (#t:Type0) (tree:tree_t t)
-requires is_tree tree 'l
-returns b:bool
-ensures is_tree tree 'l ** pure (b <==> (T.is_balanced 'l))
-{
-  match tree {
-    None -> {
-      is_tree_case_none tree;
-      true
-    }
-    Some vl -> {
-      is_tree_case_some tree vl;
-      let n = !vl;
-
-      let height_l = height n.left;
-      let height_r = height n.right;
-
-      let b1 =  (M.abs(height_r - height_l) <= 1);
-
-      let b2 = is_balanced n.right;
-
-      let b3 = is_balanced n.left;
-
-      let b4 = b1 && b2 && b3;
-      
-      intro_is_tree_node tree vl;
-      
-      b4
-    }
-  }
-}
-
-```
-
-```pulse
-fn rec  rebalance_avl (#t:Type0) (tree:tree_t t) (#l:G.erased(T.tree t))
-requires is_tree tree l
-returns y:tree_t t 
-ensures (is_tree y (T.rebalance_avl l))
-{
-  let b = is_balanced tree;
-  match tree {
-    None -> {
-      is_tree_case_none tree;
-      tree
-    }
-    Some vl -> {
-      is_tree_case_some tree vl;
-      
-      if (b)
-      {
-        intro_is_tree_node tree vl;
-        tree
-      }
-      else
-      {
-        let n = !vl;
-        let height_l = height n.left;
-        let height_r = height n.right;
-        
-        let diff_height = height_l - height_r ;
-
-        if (diff_height > 1) 
-        {
-          let vll = get_some_ref n.left;
-          intro_is_tree_node n.left vll;
-          is_tree_case_some n.left vll;
-         
-
-          let nl = !vll;
-
-          let height_ll = height nl.left;
-          let height_lr = height nl.right;
-
-          if (height_lr > height_ll)
-          {
-             (*Only in this branch, this situation happens, Node x (Node z t1 (Node y t2 t3)) t4*)
-             let vllr = get_some_ref nl.right;
-             
-             (*pack tree back in the order it is unpacked*)
-             intro_is_tree_node nl.right vllr;
-             
-             intro_is_tree_node n.left vll;
-            
-             
-             intro_is_tree_node tree vl;
-             
-             let y = rotate_left_right tree;
-             y
-          }
-          else
-          {
-            (*Node x (Node z t1 t2) t3*)
-            intro_is_tree_node n.left vll;
-            intro_is_tree_node tree vl;
-            let y = rotate_right tree;
-            y
-          }
-        }
-        else if (diff_height < -1)
-        {
-          let vlr = get_some_ref n.right;
-          intro_is_tree_node n.right vlr;
-          is_tree_case_some n.right vlr;
-         
-
-          let nr = !vlr;
-
-          let height_rl = height nr.left;
-          let height_rr = height nr.right;
-          if (height_rl > height_rr)
-          {
-             (*Node x t1 (Node z (Node y t2 t3) t4)*)
-             let vlrl = get_some_ref nr.left;
-             
-             (*pack tree back in the order it is unpacked*)
-             intro_is_tree_node nr.left vlrl;
-             intro_is_tree_node n.right vlr;
-             intro_is_tree_node tree vl;
-             let y = rotate_right_left tree;
-             y
-          }
-          else
-          {
-            (*Node x t1 (Node z t2 t3)*)
-            intro_is_tree_node n.right vlr;
-            intro_is_tree_node tree vl;
-            let y = rotate_left tree;
-            y
-          }
-          
-        }
-        else
-        {
-          intro_is_tree_node tree vl;
-          tree
-        }
-        
-      }
-    }
-  }
-}
-```
-
-```pulse
-fn rec insert_avl (#t:Type0) (cmp: T.cmp t) (tree:tree_t t) (key: t)
+fn delete_avl (#t:Type0) (cmp: T.cmp t) (tree:tree_t t) (key: t)
 requires is_tree tree 'l
 returns y:tree_t t 
-ensures (is_tree y (T.insert_avl cmp 'l key))
-{
-  match tree {
-    None -> {
-       is_tree_case_none tree;
-      
-       elim_is_tree_leaf tree;
-     
-       let left = create t;
-       let right = create t;
-      
-    
-       let y = node_cons key left right;
-      
-       let np = Some?.v y;
-      
-       is_tree_case_some y np;
-
-       intro_is_tree_node y np;
-       
-       y
-    }
-    Some vl -> {
-      is_tree_case_some tree vl;
-      let n = !vl;
-      let delta = cmp n.data key;
-      if (delta >= 0)
-      {
-        let new_left = insert_avl cmp n.left key;
-        vl := {data = n.data; left = new_left; right = n.right};
-        intro_is_tree_node (Some vl) vl #({data = n.data; left = new_left; right = n.right});
-        let new_tree = rebalance_avl (Some vl);
-        new_tree
-      }
-      else
-      {
-        let new_right = insert_avl cmp n.right key;
-        vl := {data = n.data; left = n.left; right = new_right};
-        intro_is_tree_node (Some vl) vl #({data = n.data; left = n.left; right = new_right});
-        let new_tree = rebalance_avl (Some vl);
-        new_tree
-      }
-    }
-  }
-}
-```
-```pulse //is_list_case_none$
-ghost
-fn is_tree_case_some1 (#t:Type) (x:tree_t t) (v:node_ptr t) (#ft:T.tree t) 
-requires is_tree x ft ** pure (x == Some v)
-ensures  is_tree x ft ** pure (T.Node? ft)
-{
-  cases_of_is_tree (Some v) ft;
-  unfold is_tree_cases;
-  intro_is_tree_node (Some v) v;
-}
-
-```
-
-//ensures is_tree x 'l ** pure (n == T.height 'l)
-#set-options "--print_full_names"
-
-```pulse
-fn rec tree_max_c (#t:Type0) (tree:tree_t t) (#l:G.erased(T.tree t){T.Node? l})
-requires is_tree tree l 
-returns y:t 
-ensures is_tree tree l ** pure (y == T.tree_max l)
-{
-  match tree {
-    None -> {
-      is_tree_case_none tree;
-      unreachable ()
-    }
-    Some vl -> {
-      is_tree_case_some tree vl;
-      let n = !vl;
-      let right = n.right;
-      match right {
-        None -> {
-          let d = n.data;
-          is_tree_case_none right;
-          intro_is_tree_node tree vl;
-          d
-        }
-        Some vlr -> {
-          is_tree_case_some1 right vlr;
-          let max = tree_max_c right;
-          intro_is_tree_node tree vl;
-          max
-        }
-      }
-      
-    }
-  }
-}
-```
-
-```pulse
-fn rec delete_avl (#t:Type0) (cmp: T.cmp t) (tree:tree_t t) (key: t)
-requires is_tree tree 'l
-returns y:tree_t t 
-ensures (is_tree y (T.delete_avl cmp 'l key))
+ensures emp
 {
   match tree{
    None -> {
-    is_tree_case_none tree;
-      tree
+    admit ()
    }
    Some vl -> {
     is_tree_case_some tree vl;
@@ -859,7 +92,6 @@ ensures (is_tree y (T.delete_avl cmp 'l key))
       if (delta = 0){
        let left = n.left;
        let right = n.right;
-       //explicit ltree and rtree is needed, to find a proof for the existence of func ltree and rtree
        with ltree. assert (is_tree left ltree);
        with rtree. assert (is_tree right rtree);
        match left {
@@ -868,78 +100,28 @@ ensures (is_tree y (T.delete_avl cmp 'l key))
           match right {
             None -> { (*Leaf,Leaf*)
                is_tree_case_none right #rtree;
-               let tr= create t;
-               free vl;
-               rewrite (is_tree left ltree) as (is_tree left T.Leaf);
+               assert (is_tree left ltree);
+               assert (is_tree right rtree);
+               assert (pure (ltree == T.Leaf /\ rtree == T.Leaf));
+               //
+               // AR: Without this rewrite, elim_is_tree_leaf fails
+               //
+               // rewrite (is_tree left ltree) as (is_tree left T.Leaf);
                elim_is_tree_leaf left;
-               elim_is_tree_leaf right;
-               tr
+               admit ()
             }
             Some vlr -> {(*Leaf,Node_*)
-              is_tree_case_some right vlr;
-              let rnode = !vlr;
-              vl := {data = rnode.data; left = rnode.left; right = rnode.right};
-              //rewrite each right as (Some vl);
-              intro_is_tree_node (Some vl) vl #({data = rnode.data; left = rnode.left; right = rnode.right});
-              free vlr;
-              rewrite (is_tree left ltree) as (is_tree left T.Leaf);
-              elim_is_tree_leaf left;
-              
-              //show_proof_state;
-              (Some vl)
+              admit ()
             }
           }
         }
-        Some vll -> {(*Node_,_*)
-        is_tree_case_some1 left vll;
-          match right {
-            None -> {(*Node_,Leaf*)
-              is_tree_case_some left vll;
-              is_tree_case_none right;
-              let lnode = !vll;
-              vl := {data = lnode.data; left = lnode.left; right = lnode.right};
-              //rewrite each right as (Some vl);
-              intro_is_tree_node (Some vl) vl #({data = lnode.data; left = lnode.left; right = lnode.right});
-              free vll;
-              rewrite (is_tree right rtree) as (is_tree right T.Leaf);
-              elim_is_tree_leaf right;
-              (Some vl)
-            }
-            Some vlr -> {(*Node_,Node_*)
-              //is_tree_case_some1 left vll;
-              is_tree_case_some1 right vlr;
-              let m = tree_max_c left;
-              let new_left = delete_avl cmp left m;
-              vl := {data = m; left = new_left; right = right};
-              intro_is_tree_node (Some vl) vl #({data = m; left = new_left; right = right});
-              let new_tree = rebalance_avl (Some vl);
-              assert (is_tree new_tree (T.delete_avl cmp 'l key));
-              //show_proof_state;
-              new_tree
-            }
-          }
+        _ -> {(*Node_,_*)
+        admit ()
         }
        }
       }
       else{
-        if (delta < 0) {
-          assert (pure (delta < 0));
-          let new_left = delete_avl cmp n.left key;
-          vl := {data = n.data; left = new_left; right = n.right};
-          intro_is_tree_node (Some vl) vl #({data = n.data; left = new_left; right = n.right});
-          let new_tree = rebalance_avl (Some vl);
-          new_tree
-        }
-        else{
-          let new_right = delete_avl cmp n.right key;
-          vl := {data = n.data; left = n.left; right = new_right};
-          intro_is_tree_node (Some vl) vl #({data = n.data; left = n.left; right = new_right});
-          
-          let new_tree = rebalance_avl (Some vl);
-          assert (is_tree new_tree (T.delete_avl cmp 'l key));
-          //show_proof_state;
-          new_tree
-        }
+        admit ()
       }
    }
   }
