lib/Pulse.Lib.AVLTree.fsti
@@ -1,110 +1,110 @@
 //Pulse AVL tree interface. Inspired from Steel. The FStar spec file is adopted from Steel
 //----------------------------------------------------------------------------------------------------------
 module Pulse.Lib.AVLTree
-open Pulse.Lib.Pervasives
-module S = Pulse.Lib.Stick.Util
-module FA = Pulse.Lib.Forall.Util
-open FStar.List.Tot
+// open Pulse.Lib.Pervasives
+// module S = Pulse.Lib.Stick.Util
+// module FA = Pulse.Lib.Forall.Util
+// open FStar.List.Tot
 
-module T = Spec.AVLTree
-module G = FStar.Ghost
+// module T = Spec.AVLTree
+// module G = FStar.Ghost
 
-noeq
-type node (t:Type0) = {
-    data : t;
-    left : tree_t t;
-    right : tree_t t;
-}
+// noeq
+// type node (t:Type0) = {
+//     data : t;
+//     left : tree_t t;
+//     right : tree_t t;
+// }
 
-and node_ptr (t:Type0) = ref (node t)
+// and node_ptr (t:Type0) = ref (node t)
 
-//A nullable pointer to a node
-and tree_t (t:Type0) = option (node_ptr t)
+// //A nullable pointer to a node
+// and tree_t (t:Type0) = option (node_ptr t)
 
-let vprop = slprop
+// // let vprop = slprop
 
-val is_tree #t (ct:tree_t t) (ft:T.tree t)
-: Tot vprop (decreases ft)
+// val is_tree #t (ct:tree_t t) (ft:T.tree t)
+// : Tot slprop (decreases ft)
 
-val height (#t:Type0) (x:tree_t t) (#ft:G.erased (T.tree t))
-  : stt nat
-(requires is_tree x ft)
-(ensures fun n -> is_tree x ft ** pure (n == T.height ft))
+// val height (#t:Type0) (x:tree_t t) (#ft:G.erased (T.tree t))
+//   : stt nat
+// (requires is_tree x ft)
+// (ensures fun n -> is_tree x ft ** pure (n == T.height ft))
 
-val is_empty (#t:Type) (x:tree_t t) (#ft:(T.tree t))
-   : stt bool
-  (requires is_tree x ft)
-  (ensures fun b -> is_tree x ft ** pure (b <==> (ft == T.Leaf)))
+// val is_empty (#t:Type) (x:tree_t t) (#ft:(T.tree t))
+//    : stt bool
+//   (requires is_tree x ft)
+//   (ensures fun b -> is_tree x ft ** pure (b <==> (ft == T.Leaf)))
 
-val null_tree_t (t:Type0) : tree_t t
+// val null_tree_t (t:Type0) : tree_t t
 
-val create (t:Type0)
-   : stt (tree_t t)
-  (requires emp)
-  (ensures fun x -> is_tree x T.Leaf)
+// val create (t:Type0)
+//    : stt (tree_t t)
+//   (requires emp)
+//   (ensures fun x -> is_tree x T.Leaf)
 
-val append_left_none (#t:Type0) (x:tree_t t) (v:t) (#ft:G.erased (T.tree t))
-   : stt (tree_t t)
-(requires is_tree x ft ** pure (None? x))
-(ensures fun y -> is_tree x ft  ** is_tree y (T.Node v T.Leaf T.Leaf))
+// val append_left_none (#t:Type0) (x:tree_t t) (v:t) (#ft:G.erased (T.tree t))
+//    : stt (tree_t t)
+// (requires is_tree x ft ** pure (None? x))
+// (ensures fun y -> is_tree x ft  ** is_tree y (T.Node v T.Leaf T.Leaf))
 
-val append_left (#t:Type0) (x:tree_t t) (v:t) (#ft:G.erased (T.tree t))
-   : stt (tree_t t)
-(requires is_tree x ft)
-(ensures fun y -> is_tree y  (T.append_left ft v))
+// val append_left (#t:Type0) (x:tree_t t) (v:t) (#ft:G.erased (T.tree t))
+//    : stt (tree_t t)
+// (requires is_tree x ft)
+// (ensures fun y -> is_tree y  (T.append_left ft v))
 
-val append_right (#t:Type0) (x:tree_t t) (v:t) (#ft:G.erased (T.tree t))
-   : stt (tree_t t)
-(requires is_tree x ft)
-(ensures fun y -> is_tree y  (T.append_right ft v))
+// val append_right (#t:Type0) (x:tree_t t) (v:t) (#ft:G.erased (T.tree t))
+//    : stt (tree_t t)
+// (requires is_tree x ft)
+// (ensures fun y -> is_tree y  (T.append_right ft v))
 
-val node_data (#t:Type) (x:tree_t t) (#ft:G.erased (T.tree t))
-     : stt t
-(requires is_tree x ft  ** (pure (Some? x)))
-(ensures fun _ -> is_tree x ft)
+// val node_data (#t:Type) (x:tree_t t) (#ft:G.erased (T.tree t))
+//      : stt t
+// (requires is_tree x ft  ** (pure (Some? x)))
+// (ensures fun _ -> is_tree x ft)
 
-val is_mem (#t:eqtype) (x:tree_t t) (v: t) (#ft:G.erased (T.tree t))
-     : stt bool
-(requires is_tree x ft)
-(ensures fun b -> is_tree x ft ** pure (b <==> (T.mem ft v)))
+// val is_mem (#t:eqtype) (x:tree_t t) (v: t) (#ft:G.erased (T.tree t))
+//      : stt bool
+// (requires is_tree x ft)
+// (ensures fun b -> is_tree x ft ** pure (b <==> (T.mem ft v)))
 
-val rotate_left (#t:Type0) (tree:tree_t t) (#l:G.erased(T.tree t){ Some? (T.rotate_left l) })
-     : stt (tree_t t )
-(requires is_tree tree l)
-(ensures (fun y -> is_tree y (Some?.v (T.rotate_left l))))
+// val rotate_left (#t:Type0) (tree:tree_t t) (#l:G.erased(T.tree t){ Some? (T.rotate_left l) })
+//      : stt (tree_t t )
+// (requires is_tree tree l)
+// (ensures (fun y -> is_tree y (Some?.v (T.rotate_left l))))
 
 
-val rotate_right (#t:Type0) (tree:tree_t t) (#l:G.erased (T.tree t){ Some? (T.rotate_right l) })
-    : stt (tree_t t )
-(requires is_tree tree l)
-(ensures (fun y -> is_tree y (Some?.v (T.rotate_right l))))
+// val rotate_right (#t:Type0) (tree:tree_t t) (#l:G.erased (T.tree t){ Some? (T.rotate_right l) })
+//     : stt (tree_t t )
+// (requires is_tree tree l)
+// (ensures (fun y -> is_tree y (Some?.v (T.rotate_right l))))
 
-val rotate_right_left (#t:Type0) (tree:tree_t t) (#l:G.erased (T.tree t){ Some? (T.rotate_right_left l) })
-     : stt (tree_t t )
-(requires is_tree tree l)
-(ensures (fun y -> is_tree y (Some?.v (T.rotate_right_left l))))
+// val rotate_right_left (#t:Type0) (tree:tree_t t) (#l:G.erased (T.tree t){ Some? (T.rotate_right_left l) })
+//      : stt (tree_t t )
+// (requires is_tree tree l)
+// (ensures (fun y -> is_tree y (Some?.v (T.rotate_right_left l))))
 
-val rotate_left_right (#t:Type0) (tree:tree_t t) (#l:G.erased (T.tree t){ Some? (T.rotate_left_right l) })
-     : stt (tree_t t )
-(requires is_tree tree l)
-(ensures (fun y -> is_tree y (Some?.v (T.rotate_left_right l))))
+// val rotate_left_right (#t:Type0) (tree:tree_t t) (#l:G.erased (T.tree t){ Some? (T.rotate_left_right l) })
+//      : stt (tree_t t )
+// (requires is_tree tree l)
+// (ensures (fun y -> is_tree y (Some?.v (T.rotate_left_right l))))
 
-val  is_balanced (#t:Type0) (tree:tree_t t) (#l:G.erased (T.tree t))
-     : stt bool
-(requires is_tree tree l)
-(ensures fun b -> is_tree tree l ** pure (b <==> (T.is_balanced l)))
+// val  is_balanced (#t:Type0) (tree:tree_t t) (#l:G.erased (T.tree t))
+//      : stt bool
+// (requires is_tree tree l)
+// (ensures fun b -> is_tree tree l ** pure (b <==> (T.is_balanced l)))
 
-val  rebalance_avl (#t:Type0) (tree:tree_t t) (#l: G.erased(T.tree t))
-     : stt (tree_t t )
-(requires is_tree tree l)
-(ensures fun y -> (is_tree y (T.rebalance_avl l)))
+// val  rebalance_avl (#t:Type0) (tree:tree_t t) (#l: G.erased(T.tree t))
+//      : stt (tree_t t )
+// (requires is_tree tree l)
+// (ensures fun y -> (is_tree y (T.rebalance_avl l)))
 
-val  insert_avl (#t:Type0) (cmp: T.cmp t) (tree:tree_t t) (key: t) (#l: G.erased(T.tree t))
-    : stt (tree_t t )
-(requires is_tree tree l) 
-(ensures fun y -> (is_tree y (T.insert_avl cmp l key)))
+// val  insert_avl (#t:Type0) (cmp: T.cmp t) (tree:tree_t t) (key: t) (#l: G.erased(T.tree t))
+//     : stt (tree_t t )
+// (requires is_tree tree l) 
+// (ensures fun y -> (is_tree y (T.insert_avl cmp l key)))
 
-val  delete_avl (#t:Type0) (cmp: T.cmp t) (tree:tree_t t) (key: t) (#l: G.erased(T.tree t))
-    : stt (tree_t t )
-(requires is_tree tree l) 
-(ensures fun y -> (is_tree y (T.delete_avl cmp l key)))
+// val  delete_avl (#t:Type0) (cmp: T.cmp t) (tree:tree_t t) (key: t) (#l: G.erased(T.tree t))
+//     : stt (tree_t t )
+// (requires is_tree tree l) 
+// (ensures fun y -> (is_tree y (T.delete_avl cmp l key)))
